named_api/API/context_access.v
@@ -1,5 +1,5 @@
 From NamedAPI Require Import core.
-From NamedAPI Require Import debug_functions.
+From NamedAPI Require Import context_store.
 
 (* Get and check functions for the context
 
@@ -33,65 +33,60 @@ check_ids  : nat -> list ident -> state -> bool
 
 3. Others
 -----------------------------------------------------------------
-- get_typing_context : state -> context
+- newc : state -> context
 - reduce_lets : state -> term -> term
 - reduce_except_lets :  global_env -> state -> term -> term
 - reduce_full : global_env -> state -> term -> term
 
 *)
 
-#[local] Definition ERROR_GET_SDECL : ident -> state -> state_decl :=
-  fun id s => let ERR_MSG := "ERROR_GET_SDECL:" ^ id in
-              mk_sdecl ERR_MSG
-              (mkdecl (mkBindAnn (nNamed ERR_MSG) Relevant)
-              (Some (state_to_term s)) (state_to_term s)).
 
 (* 1.0 Local functions geting term and type with shifted *)
-#[local] Definition get_sdecl : ident -> state -> (nat * state_decl) :=
-  fun id s =>
-  let fix aux n s' :=
-  match s' with
-  | [] => (0, ERROR_GET_SDECL id s)
-  | sdecl :: s' => if eqb id sdecl.(state_name) then (n, sdecl) else aux (S n) s'
-  end in
-  aux 0 s.(state_context).
+Definition lift_cdecl : nat -> context_decl -> context_decl :=
+  fun n ' (mkdecl an x ty) => mkdecl an (option_map (lift0 n) x) (lift0 n ty).
+
+#[local] Definition ERROR_CDECL : context_decl :=
+  mkdecl (mkBindAnn nAnon Relevant) None (tVar "error_get_sdecl").
+
+#[local] Definition get_decl : state -> key -> context_decl :=
+  fun s k =>
+  let n' := length (newc s) - k -1 in
+  lift_cdecl n' (nth n' (newc s) ERROR_CDECL).
 
 Section Get.
 
   Context {X : Type}.
-  Context (f : nat -> state_decl -> X).
+  Context (f : nat -> context_decl -> X).
 
-  Definition concat_strings : list string -> string :=
-    fun l => fold_right (fun s t => s ^ " " ^ t) "" l.
+  #[local] Definition geti_key: keys -> nat -> key :=
+    fun ks pos1 => nth pos1 ks 200.
 
-  #[local] Definition get_id1: list ident -> nat -> ident :=
-    fun ids pos1 => nth pos1 ids ("ERROR GET_ID1: " ^ (concat_strings ids)).
+  #[local] Definition getij_key : list keys -> nat -> nat -> key :=
+  fun kss pos1 pos2 =>
+  let ks := nth pos1 kss [] in
+  nth pos2 ks 200.
 
-  #[local] Definition get_id2 : list (list ident) -> nat -> nat -> ident :=
-  fun idss pos1 pos2 =>
-  let ids := nth pos1 idss ["ERROR GET_ID2: nth pos1"] in
-  nth pos2 ids "ERROR GET_ID2: nth pos2".
+  #[local] Definition get_X : state -> key -> X :=
+    fun s k => f (#|newc s| - k -1) (get_decl s k).
 
-  #[local] Definition get_X : ident -> state -> X :=
-    fun id s => let ' (pos_var, sdecl) := get_sdecl id s in f pos_var sdecl.
+  #[local] Definition geti_X : state -> keys -> nat -> X :=
+      fun s ks pos_k => get_X s (geti_key ks pos_k).
 
-  #[local] Definition geti_X : list ident -> nat -> state -> X :=
-      fun ids pos_id s => get_X (get_id1 ids pos_id) s.
+  #[local] Definition getij_X : state -> list keys -> nat -> nat -> X :=
+  fun s kss pos_k1 pos_k2 => get_X s (getij_key kss pos_k1 pos_k2).
 
-  #[local] Definition getij_X : list (list ident) -> nat -> nat -> state -> X :=
-  fun ids pos_id1 pos_id2 s => get_X (get_id2 ids pos_id1 pos_id2) s.
-
-  #[local] Definition get_Xs : list ident -> state -> list X :=
-  fun l s => map (fun x => get_X x s) l.
+  #[local] Definition get_Xs : state -> keys -> list X :=
+  fun s ks => map (fun k => get_X s k) ks.
 
 End Get.
 
+
 (* 1.1 Get terms *)
-#[local] Definition get_sdecl_term : nat -> state_decl -> term :=
-  fun shift ' (mk_sdecl _ (mkdecl _ bd _)) =>
+#[local] Definition get_sdecl_term : nat -> context_decl -> term :=
+  fun n ' (mkdecl _ bd _) =>
   match bd with
-  | Some tm => lift0 (S shift) tm
-  | None => tRel shift
+  | Some tm => lift0 1 tm
+  | None => tRel n
   end.
 
 Definition get_term := get_X get_sdecl_term.
@@ -100,8 +95,8 @@ Definition getij_term := getij_X get_sdecl_term.
 Definition get_terms := get_Xs get_sdecl_term.
 
 (* 1.2 Get types *)
-#[local] Definition get_sdecl_type : nat -> state_decl -> term :=
-  fun shift ' (mk_sdecl _ (mkdecl _ _ ty)) => lift0 (S shift) ty.
+#[local] Definition get_sdecl_type : nat -> context_decl -> term :=
+  fun _ ' (mkdecl _ _ ty) => lift0 1 ty.
 
 Definition get_type   := get_X   get_sdecl_type.
 Definition geti_type  := geti_X  get_sdecl_type.
@@ -109,74 +104,67 @@ Definition getij_type := getij_X get_sdecl_type.
 Definition get_types  := get_Xs  get_sdecl_type.
 
 (* 1.3 Get aname *)
-#[local] Definition get_sdecl_aname : nat -> state_decl -> aname :=
-  fun _ sdecl => sdecl.(state_def).(decl_name).
+#[local] Definition get_sdecl_aname : nat -> context_decl -> aname :=
+  fun _ cdecl => cdecl.(decl_name).
 
 Definition get_aname   := get_X   get_sdecl_aname.
 Definition geti_aname  := geti_X  get_sdecl_aname.
 Definition getij_aname := getij_X get_sdecl_aname.
 Definition get_anames  := get_Xs  get_sdecl_aname.
 
-(* 1.4 Check *)
-Definition get_pos : ident -> state -> nat :=
-  fun id s => let ' (n, _) := get_sdecl id s in n.
 
-Definition check_pos: ident -> nat -> state -> bool :=
-  fun id read_pos s => let ' (pos_cxt, _) := get_sdecl id s in eqb pos_cxt read_pos.
+(* 1.4 Check *)
+Definition get_pos : state -> key -> nat :=
+  fun s k => #|newc s| -k -1.
+
+Definition check_pos: state -> key -> nat -> bool :=
+  fun s k read_pos => eqb (#|newc s| -k -1) read_pos.
 
 
 
 (* 2. Access by position *)
-#[local] Definition ERROR_GETP_SDECL : nat -> state -> state_decl :=
-  fun pos s => mk_sdecl "ERROR GET SDECL"
-              (mkdecl (mkBindAnn (nNamed ("ERROR_GET_SDECL: " ^ string_of_nat pos)) Relevant)
-              (Some (tVar "ERROR GET SDECL")) (tVar "ERROR GET SDECL")).
 
-#[local] Definition getp_sdecl : nat -> state -> state_decl :=
-  fun pos s => nth pos s.(state_context) (ERROR_GETP_SDECL pos s).
+#[local] Definition getp_cdecl : state -> nat -> context_decl :=
+  fun s pos => nth pos s.(state_context) ERROR_CDECL.
 
-Definition getp_name : nat -> state -> ident :=
-  fun pos s => (getp_sdecl pos s).(state_name).
+Definition getp_key : state -> nat -> key :=
+  fun s pos => pos.
 
-Definition getp_aname : nat -> state -> aname :=
-  fun pos s => (getp_sdecl pos s).(state_def).(decl_name).
+Definition getp_aname : state -> nat -> aname :=
+  fun s pos => (getp_cdecl s pos).(decl_name).
 
-Definition getp_body : nat -> state -> option term :=
-  fun pos s => (getp_sdecl pos s).(state_def).(decl_body).
+Definition getp_body : state -> nat ->  option term :=
+  fun s pos => (getp_cdecl s pos).(decl_body).
 
-Definition getp_type : nat -> state -> term :=
-  fun pos s => (getp_sdecl pos s).(state_def).(decl_type).
+Definition getp_type : state -> nat -> term :=
+  fun s pos => (getp_cdecl s pos).(decl_type).
 
-Definition check_id : nat -> ident -> state -> bool :=
-  fun pos id s => eqb (state_name (getp_sdecl pos s)) id.
+Definition check_key : state -> key -> nat -> bool :=
+  fun s k pos => eqb (#|newc s| -k -1) (getp_key s pos).
 
-Definition check_ids : nat -> list ident -> state -> bool :=
-  fun pos ids s => fold_right (fun id t => (check_id pos id s) || t) false ids.
-
+Definition check_keys : state -> keys -> nat -> bool :=
+  fun s ks pos => fold_right (fun k c => (check_key s k pos) || c) false ks.
 
 
 (* 3. Others *)
-Definition get_typing_context : state -> context :=
-  fun s => map state_def s.(state_context).
-
 From MetaCoq Require Import Template.Checker.
 Import RedFlags.
 
 #[local] Definition noiota_flags := mk true true false true true true.
 
 Definition reduce_lets : state -> term -> term :=
-  fun s t => expand_lets (get_typing_context s) t.
+  fun s t => expand_lets (newc s) t.
 
 Definition reduce_except_lets :  global_env -> state -> term -> term :=
   fun E s t =>
-  match reduce_opt noiota_flags E (get_typing_context s) 5000 t with
+  match reduce_opt noiota_flags E (newc s) 5000 t with
   | Some t => t
   | None => tVar "ERREUR REDUCTION"
   end.
 
 Definition reduce_full : global_env -> state -> term -> term :=
   fun E s t =>
-  match reduce_opt default E (get_typing_context s) 5000 t with
+  match reduce_opt default E (newc s) 5000 t with
   | Some t => t
   | None => tVar "ERREUR REDUCTION"
   end.
