named_api/API/context_store.v
@@ -17,57 +17,136 @@ From NamedAPI Require Import fold_functions.
 Notation "let* x .. z ':=' c1 'in' c2" := (c1 (fun x => .. (fun z => c2) ..))
 (at level 100, x binder, z binder, c1 at next level, right associativity).
 
-
-#[local] Definition fresh_ident_aux : option ident -> nat -> ident :=
-  fun x k => match x with
-  | Some s => s     ^ "#" ^ (string_of_nat k)
-  | None   => "Var" ^ "#" ^ (string_of_nat k)
-  end.
-
-Definition fresh_ident : option ident -> state -> ident :=
-  fun x s => fresh_ident_aux x (length s.(state_context)).
+Definition key := nat.
+Definition keys := list nat.
+Definition fresh_key : state -> key :=
+  fun s => #|s.(state_context)|.
 
 #[local] Definition lift1 : list term -> list term :=
     map (lift0 1).
 
-(* Add a previously existing var to the current context *)
-Definition add_old_var {X} : option ident -> context_decl -> state -> (ident -> state -> X) -> X :=
-  fun x cdecl s t =>
-    let id := fresh_ident x s in
-    let updated_cdecl := weaken_decl s cdecl in
-    let s := mk_state (mk_sdecl id updated_cdecl :: s.(state_context))
-                ((tRel 0) :: lift1 s.(state_subst)) s.(state_ind) in
-    t id s.
 
-Definition add_old_context {X} : option ident -> context -> state ->
-    (list ident -> list ident -> list ident -> state -> X) -> X :=
-  fun x => fold_left_state_opt3
-    ( fun _ cdecl s t =>
-      match cdecl.(decl_body) with
-      | Some db => let* id_let s := add_old_var x cdecl s in
-                   t [id_let] [] [id_let] s
-      | None    => let* id_arg s := add_old_var x cdecl s in
-                   t [] [id_arg] [id_arg] s
+
+
+(* 1. Add existing var / letin / context *)
+
+Definition add_ovar (s : state) (x : option ident) (an : aname) (ty : term) : state :=
+  mk_state (newc s ,, vass an (weaken s ty))
+           (state_context_debug s ,, x)
+           (lift1 s.(state_subst),, tRel 0)
+           (state_inds s).
+
+Definition add_old_var {X} : state -> option ident -> aname -> term -> (state -> key -> X) -> X :=
+fun s x an ty cc =>
+  let s' := add_ovar s x an ty in
+  cc s' (fresh_key s).
+
+
+Definition add_oletin (s : state) (x : option ident) (an : aname) (db : term) (ty : term) : state :=
+mk_state (newc s ,, vdef an (weaken s db) (weaken s ty))
+         (state_context_debug s ,, x)
+         (lift1 s.(state_subst),, tRel 0)
+         (state_inds s).
+
+Definition add_old_letin {X} : state -> option ident -> aname -> term -> term -> (state -> key -> X) -> X :=
+  fun s x an db ty cc =>
+    let s' := add_oletin s x an db ty in
+    cc s' (fresh_key s).
+
+
+Definition add_ocontext (s : state) (x : option ident) (cxt : context) : state :=
+  fold_right (fun ' (mkdecl an z ty) s =>
+    match z with
+    | None => add_ovar s x an ty
+    | Some db => add_oletin s x an db ty
+    end) s cxt.
+
+(* To rebuild on top of add_ocontext to make dependent *)
+Definition add_old_context {X} : state -> option ident -> context ->
+    (state -> keys -> keys -> keys -> X) -> X :=
+  fun s x cxt => fold_left_state_opt3
+    ( fun _ ' (mkdecl an z ty) s cc =>
+      match z with
+      | Some db => let* s id_let := add_old_letin s x an db ty in
+                   cc s [id_let] [] [id_let]
+      | None    => let* s id_arg := add_old_var s x an ty in
+                   cc s [] [id_arg] [id_arg]
       end
-  ).
+  ) cxt s.
 
-(* Add a fresh var to the current context *)
-Definition add_fresh_var {X} : option ident -> context_decl -> state -> (ident -> state -> X) -> X :=
-  fun x cdecl s t =>
-  let id := fresh_ident x s in
-  let s := mk_state (mk_sdecl id cdecl :: s.(state_context))
-            (lift1 s.(state_subst)) s.(state_ind) in
-  t id s.
 
-(* Add a fresh context to the current context *)
-Definition add_fresh_context {X} : option ident -> context -> state -> (list ident -> state -> X) -> X :=
-  fun x cxt s t => fold_left_state (fun _ cdecl s t => add_fresh_var x cdecl s t) cxt s t.
 
-(* Remove a previously existing var by substituting it *)
-Definition subst_old_var {X} : term -> state -> (state -> X) -> X :=
-  fun tm ' (mk_state cxt subst inds) t => t (mk_state cxt (tm :: subst) inds).
 
-(* Remove n previously existing var by substituting them *)
-Definition subst_old_vars {X} : list term -> state -> (state -> X) -> X :=
-  fun ltm ' (mk_state cxt subst inds) t => t (mk_state cxt (rev ltm ++ subst) inds).
+(* 2. Add fresh var / letin / context *)
+
+Definition add_fvar (s : state) (x : option ident) (an : aname) (ty : term) : state :=
+  mk_state (newc s ,, vass an ty)
+           (state_context_debug s ,, x)
+           (lift1 s.(state_subst))
+           (state_inds s).
+
+Definition add_fresh_var {X} : state -> option ident -> aname -> term -> (state -> key -> X) -> X :=
+  fun s x an ty cc =>
+  let s' := add_fvar s x an ty in
+  cc s' (fresh_key s).
+
+
+Definition add_fletin (s : state) (x : option ident) (an : aname) (db : term) (ty : term) : state :=
+  mk_state (newc s ,, vdef an db ty)
+            (state_context_debug s ,, x)
+            (lift1 s.(state_subst))
+            (state_inds s).
+
+Definition add_fresh_letin {X} : state -> option ident -> aname -> term -> term -> (state -> key -> X) -> X :=
+  fun s x an db ty cc =>
+  let s' := add_fletin s x an db ty in
+  cc s' (fresh_key s).
+
+
+Definition add_fcontext (s : state) (x : option ident) (cxt : context) : state :=
+  fold_right (fun ' (mkdecl an z ty) s =>
+    match z with
+    | None => add_fvar s x an ty
+    | Some db => add_fletin s x an db ty
+    end) s cxt.
+
+(* To rebuild on top of add_fcontext to make dependent *)
+Definition add_fresh_context {X} : state -> option ident -> context ->
+    (state -> keys -> keys -> keys -> X) -> X :=
+  fun s x cxt => fold_left_state_opt3
+    (fun _ ' (mkdecl an z ty) s cc =>
+      match z with
+      | Some db => let* s id_let := add_fresh_letin s x an db ty  in
+                   cc s [id_let] [] [id_let]
+      | None    => let* s id_arg := add_fresh_var s x an ty in
+                   cc s [] [id_arg] [id_arg]
+      end
+  ) cxt s.
+
+
+
+
+(* 3. Substitute existing var / letin / context *)
+(* To rebuild to make dependent *)
+Definition subst_obind (s : state) (tm : term) : state :=
+  mk_state (newc s)
+           (state_context_debug s)
+           (tm :: lift1 s.(state_subst))
+           (state_inds s).
+
+Definition subst_old_bind {X} : state -> term -> (state -> X) -> X :=
+  fun s tm cc =>
+  let s' := subst_obind s tm in
+  cc s'.
+
+Definition subst_ocontext (s : state) (ltm : list term) : state :=
+  mk_state (newc s)
+  (state_context_debug s)
+  (rev ltm ++ map (lift0 #|ltm|) s.(state_subst))
+  (state_inds s).
+
+Definition subst_old_context {X} : state -> list term -> (state -> X) -> X :=
+  fun s ltm cc =>
+  let s' := subst_ocontext s ltm in
+  cc s'.
 
