named_api/API/fold_functions.v
@@ -17,96 +17,96 @@ Export ListNotations.
 
 
 (* 1.1 Fold_left and Fold_right *)
-Definition fold_right_state {A B X state} (tp : nat -> A -> state -> (X -> state -> B) -> B)
-  (l:list A) (s:state) (t : list X -> state -> B) : B :=
+Definition fold_right_state {A B X state} (tp : nat -> A -> state -> (state -> X -> B) -> B)
+  (l:list A) (s:state) (t : state -> list X -> B) : B :=
   let fix aux n ids1 l s t : B :=
     match l with
-    | [] => t (rev ids1) s
-    | a :: l => tp n a s (fun id1 s => aux (S n) (id1 :: ids1) l s t)
+    | [] => t s (rev ids1)
+    | a :: l => tp n a s (fun s id1 => aux (S n) (id1 :: ids1) l s t)
   end in
   aux 0 [] l s t.
 
-  Definition fold_right_state2 {A B X Y state} (tp : nat -> A -> state -> (X -> Y -> state -> B) -> B)
-  (l:list A) (s:state) (t : list X -> list Y -> state -> B) : B :=
+  Definition fold_right_state2 {A B X Y state} (tp : nat -> A -> state -> (state -> X -> Y -> B) -> B)
+  (l:list A) (s:state) (t : state -> list X -> list Y -> B) : B :=
   let fix aux n ids1 ids2 l s t : B :=
     match l with
-    | [] => t (rev ids1) (rev ids2) s
-    | a :: l => tp n a s (fun id1 id2 s => aux (S n) (id1 :: ids1) (id2 :: ids2) l s t)
+    | [] => t s (rev ids1) (rev ids2)
+    | a :: l => tp n a s (fun s id1 id2 => aux (S n) (id1 :: ids1) (id2 :: ids2) l s t)
   end in
   aux 0 [] [] l s t.
 
-Definition fold_right_state3 {A B X Y Z state} (tp : nat -> A -> state -> (X -> Y -> Z -> state -> B) -> B)
-  (l:list A) (s:state) (t : list X -> list Y -> list Z -> state -> B) : B :=
+Definition fold_right_state3 {A B X Y Z state} (tp : nat -> A -> state -> (state -> X -> Y -> Z -> B) -> B)
+  (l:list A) (s:state) (t : state -> list X -> list Y -> list Z -> B) : B :=
   let fix aux n ids1 ids2 ids3 l s t : B :=
     match l with
-    | [] => t (rev ids1) (rev ids2) (rev ids3) s
-    | a :: l => tp n a s (fun id1 id2 id3 s => aux (S n) (id1 :: ids1) (id2 :: ids2) (id3 :: ids3) l s t)
+    | [] => t s (rev ids1) (rev ids2) (rev ids3)
+    | a :: l => tp n a s (fun s id1 id2 id3 => aux (S n) (id1 :: ids1) (id2 :: ids2) (id3 :: ids3) l s t)
   end in
   aux 0 [] [] [] l s t.
 
-Definition fold_left_state {A B X state} (tp : nat -> A -> state -> (X -> state -> B) -> B)
-  (l:list A) (s:state) (t : list X -> state -> B) : B :=
+Definition fold_left_state {A B X state} (tp : nat -> A -> state -> (state -> X -> B) -> B)
+  (l:list A) (s:state) (t : state -> list X -> B) : B :=
   fold_right_state tp (rev l) s t.
 
-Definition fold_left_state2 {A B X Y state} (tp : nat -> A -> state -> (X -> Y -> state -> B) -> B)
-  (l:list A) (s:state) (t : list X -> list Y -> state -> B) : B :=
+Definition fold_left_state2 {A B X Y state} (tp : nat -> A -> state -> (state -> X -> Y -> B) -> B)
+  (l:list A) (s:state) (t : state -> list X -> list Y -> B) : B :=
   fold_right_state2 tp (rev l) s t.
 
-Definition fold_left_state3 {A B X Y Z state} (tp : nat -> A -> state -> (X -> Y -> Z -> state -> B) -> B)
-  (l:list A) (s:state) (t : list X -> list Y -> list Z -> state -> B) : B :=
+Definition fold_left_state3 {A B X Y Z state} (tp : nat -> A -> state -> (state -> X -> Y -> Z -> B) -> B)
+  (l:list A) (s:state) (t : state -> list X -> list Y -> list Z -> B) : B :=
   fold_right_state3 tp (rev l) s t.
 
 (* 1.2 Fold_right and Fold_left conditional *)
-Definition fold_right_state_opt {A B X state} (tp : nat -> A -> state -> (list X -> state -> B) -> B)
-  (l:list A) (s:state) (t : list X -> state -> B) : B :=
+Definition fold_right_state_opt {A B X state} (tp : nat -> A -> state -> (state -> list X -> B) -> B)
+  (l:list A) (s:state) (t : state -> list X -> B) : B :=
   let fix aux n ids1 l s t : B :=
     match l with
-    | [] => t (rev ids1) s
-    | a :: l => tp n a s (fun fid1 s => aux (S n) (fid1 ++ ids1) l s t)
+    | [] => t s (rev ids1)
+    | a :: l => tp n a s (fun s fid1 => aux (S n) (fid1 ++ ids1) l s t)
   end in
   aux 0 [] l s t.
 
-Definition fold_right_state_opt2 {A B X Y state} (tp : nat -> A -> state -> (list X -> list Y -> state -> B) -> B)
-  (l:list A) (s:state) (t : list X -> list Y -> state -> B) : B :=
+Definition fold_right_state_opt2 {A B X Y state} (tp : nat -> A -> state -> (state -> list X -> list Y -> B) -> B)
+  (l:list A) (s:state) (t : state -> list X -> list Y -> B) : B :=
   let fix aux n ids1 ids2 l s t : B :=
     match l with
-    | [] => t (rev ids1) (rev ids2) s
-    | a :: l => tp n a s (fun fid1 fid2 s => aux (S n) (fid1 ++ ids1) (fid2 ++ ids2) l s t)
+    | [] => t s (rev ids1) (rev ids2)
+    | a :: l => tp n a s (fun s fid1 fid2 => aux (S n) (fid1 ++ ids1) (fid2 ++ ids2) l s t)
   end in
   aux 0 [] [] l s t.
 
-Definition fold_right_state_opt3 {A B X Y Z state} (tp : nat -> A -> state -> (list X -> list Y -> list Z -> state -> B) -> B)
-  (l:list A) (s:state) (t : list X -> list Y -> list Z -> state -> B) : B :=
+Definition fold_right_state_opt3 {A B X Y Z state} (tp : nat -> A -> state -> (state -> list X -> list Y -> list Z -> B) -> B)
+  (l:list A) (s:state) (t : state -> list X -> list Y -> list Z -> B) : B :=
   let fix aux n ids1 ids2 ids3 l s t : B :=
     match l with
-    | [] => t (rev ids1) (rev ids2) (rev ids3) s
-    | a :: l => tp n a s (fun fid1 fid2 fid3 s => aux (S n) (fid1 ++ ids1) (fid2 ++ ids2) (fid3 ++ ids3) l s t)
+    | [] => t s (rev ids1) (rev ids2) (rev ids3)
+    | a :: l => tp n a s (fun s fid1 fid2 fid3 => aux (S n) (fid1 ++ ids1) (fid2 ++ ids2) (fid3 ++ ids3) l s t)
   end in
   aux 0 [] [] [] l s t.
 
-Definition fold_right_state_opt4 {A B X Y Z W state} (tp : nat -> A -> state -> (list X -> list Y -> list Z -> list W -> state -> B) -> B)
-  (l:list A) (s:state) (t : list X -> list Y -> list Z -> list W -> state -> B) : B :=
+Definition fold_right_state_opt4 {A B X Y Z W state} (tp : nat -> A -> state -> (state -> list X -> list Y -> list Z -> list W -> B) -> B)
+  (l:list A) (s:state) (t : state -> list X -> list Y -> list Z -> list W -> B) : B :=
   let fix aux n ids1 ids2 ids3 ids4 l s t : B :=
     match l with
-    | [] => t (rev ids1) (rev ids2) (rev ids3) (rev ids4) s
-    | a :: l => tp n a s (fun fid1 fid2 fid3 fid4 s =>
+    | [] => t s (rev ids1) (rev ids2) (rev ids3) (rev ids4)
+    | a :: l => tp n a s (fun s fid1 fid2 fid3 fid4 =>
           aux (S n) (fid1 ++ ids1) (fid2 ++ ids2) (fid3 ++ ids3) (fid4 ++ ids4) l s t)
   end in
   aux 0 [] [] [] [] l s t.
 
-Definition fold_left_state_opt {A B X state} (tp : nat -> A -> state -> (list X -> state -> B) -> B)
-  (l:list A) (s:state) (t : list X -> state -> B) : B :=
+Definition fold_left_state_opt {A B X state} (tp : nat -> A -> state -> (state -> list X -> B) -> B)
+  (l:list A) (s:state) (t : state -> list X -> B) : B :=
   fold_right_state_opt tp (rev l) s t.
 
-Definition fold_left_state_opt2 {A B X Y state} (tp : nat -> A -> state -> (list X -> list Y -> state -> B) -> B)
-  (l:list A) (s:state) (t : list X -> list Y -> state -> B) : B :=
+Definition fold_left_state_opt2 {A B X Y state} (tp : nat -> A -> state -> (state -> list X -> list Y -> B) -> B)
+  (l:list A) (s:state) (t : state -> list X -> list Y -> B) : B :=
   fold_right_state_opt2 tp (rev l) s t.
 
-Definition fold_left_state_opt3 {A B X Y Z state} (tp : nat -> A -> state -> (list X -> list Y -> list Z -> state -> B) -> B)
-  (l:list A) (s:state) (t : list X -> list Y -> list Z -> state -> B) : B :=
+Definition fold_left_state_opt3 {A B X Y Z state} (tp : nat -> A -> state -> (state -> list X -> list Y -> list Z -> B) -> B)
+  (l:list A) (s:state) (t : state -> list X -> list Y -> list Z -> B) : B :=
   fold_right_state_opt3 tp (rev l) s t.
 
-Definition fold_right_state_op4t {A B X Y Z W state} (tp : nat -> A -> state -> (list X -> list Y -> list Z -> list W -> state -> B) -> B)
-  (l:list A) (s:state) (t : list X -> list Y -> list Z -> list W -> state -> B) : B :=
+Definition fold_right_state_op4t {A B X Y Z W state} (tp : nat -> A -> state -> (state -> list X -> list Y -> list Z -> list W -> B) -> B)
+  (l:list A) (s:state) (t : state -> list X -> list Y -> list Z -> list W -> B) : B :=
   fold_right_state_opt4 tp (rev l) s t.
 
