named_api/Functoriality/functoriality_rec_call.v
@@ -14,10 +14,10 @@ let fix aux n l :=
   end in
   aux 0 l.
 
-Definition make_ind' : kername -> nat -> list ident -> list term -> list term -> state -> term :=
-  fun kname pos_indb id_uparams nuparams indices s =>
+Definition make_ind' : state -> kername -> nat -> keys -> list term -> list term -> term :=
+  fun s kname pos_indb key_uparams nuparams indices =>
   mkApps (tInd (mkInd kname pos_indb) [])
-          ( get_terms id_uparams s ++ nuparams ++ indices).
+          (get_terms s key_uparams ++ nuparams ++ indices).
 
 
 (* 1. Instiates Parametricity with rec call *)
@@ -36,8 +36,8 @@ Fixpoint one_replace_list {A} (pos : nat) (a : A) (l : list A) : list A :=
 Definition replace_list {A} (lpos : list nat) (la : list A) (l : list A) : list A :=
   fold_right (fun ' (pos, a) t => one_replace_list pos a t) l (combine lpos la).
 
-Definition sub : list ident -> list term -> state -> list term :=
-  fun ids rp s => replace_list (map (fun x => get_pos x s) ids) rp (triv_subst s).
+Definition sub : state -> keys -> list term -> list term :=
+  fun s ks rp => replace_list (map (fun x => get_pos s x) ks) rp (triv_subst s).
 
 
 (* 2. Generates rec call for inductive *)
@@ -45,45 +45,46 @@ Unset Guard Checking.
 
 Section MkRecCall.
 
-(* Context (make_indp : nat -> list ident -> list term -> list term -> state -> term). *)
+(* Context (make_indp : nat -> keys -> list term -> list term -> state -> term). *)
 Context (kname : kername).
 Context (Ep : param_env).
-Context (id_uparams    : list ident).
-Context (id_spuparams  : list ident).
-Context (id_uparam_bis : list ident).
-Context (id_funcs      : list ident).
-Context (id_fixs       : list ident).
+Context (s : state).
+Context (key_uparams    : keys).
+Context (key_spuparams  : keys).
+Context (key_uparam_bis : keys).
+Context (key_funcs      : keys).
+Context (key_fixs       : keys).
 
-Definition sub_bis s := sub id_uparams (get_terms id_uparam_bis s) s.
+Definition sub_bis s := sub s key_uparams (get_terms s key_uparam_bis).
 
-Fixpoint add_param (strpos : list bool) (l : list term) (rc : list term) (s : state) : list term :=
+Fixpoint add_param (s : state) (strpos : list bool) (l : list term) (rc : list term) : list term :=
   match strpos, l, rc with
   | nil, nil, nil => nil
-  | true :: strpos, A::l, tm :: rc => A :: (subst0 (sub_bis s) A) :: tm :: (add_param strpos l rc s)
-  | false :: strpos, A::l, x :: rc => A :: (add_param strpos l rc s)
+  | true :: strpos, A::l, tm :: rc => A :: (subst0 (sub_bis s) A) :: tm :: (add_param s strpos l rc)
+  | false :: strpos, A::l, x :: rc => A :: (add_param s strpos l rc)
   | _, _, _ => nil
 end.
 
-Fixpoint make_func_call_aux (id_arg : ident) (rev_ids_local : list ident) (ty : term) (s : state) {struct ty} : term :=
+Fixpoint make_func_call_aux (s : state) (key_arg : key) (rev_ids_local : keys) (ty : term) {struct ty} : term :=
   let (hd, iargs) := decompose_app ty in
   match hd with
   (* 1. If it is an iterated product or LetIn => accumulates arg  *)
   | tProd an A B =>
-      let* id_local s := add_old_var (Some "local_arg") (mkdecl an None A) s in
-      let tm := make_func_call_aux id_arg (id_local :: rev_ids_local) B s in
+      let* s key_local := add_old_var s (Some "local_arg") an A in
+      let tm := make_func_call_aux s key_arg (key_local :: rev_ids_local) B in
       tLambda an A tm
   | tLetIn an db A B =>
-      let* _ s := add_old_var (Some "local_let") (mkdecl an (Some db) A) s in
-      let tm := make_func_call_aux id_arg rev_ids_local B s in
+      let* s _ := add_old_letin s (Some "local_let") an db A in
+      let tm := make_func_call_aux s key_arg rev_ids_local B in
       tLetIn an db A tm
   (* 2. If it an strictly postive uniform parameter *)
   | tRel n =>
-      match find_bool (fun id => check_pos id n s) id_spuparams with
+      match find_bool (fun k => check_pos s k n) key_spuparams with
       | (pos_func, true) =>
-            mkApp (geti_term id_funcs pos_func s)
-                  (mkApps (get_term id_arg s)
-                          (get_terms (rev rev_ids_local) s))
-      | (pos_param, false) => mkApps (get_term id_arg s) (get_terms (rev rev_ids_local) s)
+            mkApp (geti_term s key_funcs pos_func)
+                  (mkApps (get_term s key_arg)
+                          (get_terms s (rev rev_ids_local)))
+      | (pos_param, false) => mkApps (get_term s key_arg) (get_terms s (rev rev_ids_local))
       end
   (* 3. If it is an inductive *)
   | tInd (mkInd kname_indb pos_indb) _ =>
@@ -92,12 +93,12 @@ Fixpoint make_func_call_aux (id_arg : ident) (rev_ids_local : list ident) (ty : 
     then let nuparams_indices := skipn (get_nb_uparams kname s) iargs in
          let nuparams := firstn (get_nb_nuparams kname s) nuparams_indices in
          let indices  := skipn  (get_nb_nuparams kname s) nuparams_indices in
-          mkApp (mkApps (geti_term id_fixs pos_indb s) (nuparams ++ indices))
-                (mkApps (get_term id_arg s)
-                        (get_terms (rev rev_ids_local) s))
+          mkApp (mkApps (geti_term s key_fixs pos_indb) (nuparams ++ indices))
+                (mkApps (get_term  s key_arg)
+                        (get_terms s (rev rev_ids_local)))
     (* 3.2 If it is nested *)
     else if length iargs =? 0
-    then mkApps (get_term id_arg s) (get_terms (rev rev_ids_local) s)
+    then mkApps (get_term s key_arg) (get_terms s (rev rev_ids_local))
     else match find (fun x => eq_constant kname_indb x.(ep_kname)) Ep with
       | Some xp =>
         (* 3.2.1 get uparams and nuparams + indices *)
@@ -106,26 +107,26 @@ Fixpoint make_func_call_aux (id_arg : ident) (rev_ids_local : list ident) (ty : 
         (* 3.2.2 Check for further rec call recursively *)
         let compute_nested_rc (x : term) (s s : state) : term :=
           let anx := mkBindAnn nAnon Relevant in
-          let* id_farg s := add_fresh_var (Some "rec_arg") (mkdecl anx None x) s in
-          let tm := make_func_call_aux id_farg [] (lift0 1 x) s in
+          let* s key_farg := add_fresh_var s (Some "rec_arg") anx x in
+          let tm := make_func_call_aux s key_farg [] (lift0 1 x) in
           tLambda anx x tm
         in
         let rec_call := map (fun x => compute_nested_rc x s s) uparams_indb in
-        let ltm := add_param xp.(ep_strpos_uparams) uparams_indb rec_call s in
+        let ltm := add_param s xp.(ep_strpos_uparams) uparams_indb rec_call in
         (* mkApp (state_to_term s) (mkApps (tVar "Subst: ") (sub_bis s)) *)
         mkApp (mkApps (tConst xp.(ep_func_kname) [])
                       (ltm ++ nuparams_indices_indb))
-              (mkApps (get_term id_arg s)
-                      (get_terms (rev rev_ids_local) s))
+              (mkApps (get_term  s key_arg)
+                      (get_terms s (rev rev_ids_local)))
           (* Otherwise, kill the branch *)
-      | None => mkApps (get_term id_arg s) (get_terms (rev rev_ids_local) s)
+      | None => mkApps (get_term s key_arg) (get_terms s (rev rev_ids_local))
       end
   (* 4. Otherwise *)
-  | _ => mkApps (get_term id_arg s) (get_terms (rev rev_ids_local) s)
+  | _ => mkApps (get_term s key_arg) (get_terms s (rev rev_ids_local))
   end.
 
 #[using="All"]
-Definition make_func_call : ident -> term -> state -> term :=
-  fun id_arg ty s => make_func_call_aux id_arg [] ty s.
+Definition make_func_call : key -> term -> term :=
+  fun key_arg ty => make_func_call_aux s key_arg [] ty.
 
 End MkRecCall.
