named_api/Preprocess/strictly_positive_uniform_parameters.v
@@ -74,30 +74,30 @@ Section CustomParam.
 
   (* 2. Compute strict pos for an arg *)
 Section CheckArg.
-  Context (id_inds   : list ident).
-  Context (id_uparams : list ident).
-  Context (id_nuparams : list ident).
+  Context (key_inds     : keys).
+  Context (key_uparams  : keys).
+  Context (key_nuparams : keys).
 
-  Definition check_not_free (ty : term) (s : state) : list bool :=
+  Definition check_not_free (s : state) (ty : term) : list bool :=
     map (fun pos => noccur_between pos 1 ty)
-        (map get_rel (get_terms id_uparams s)).
+        (map get_rel (get_terms s key_uparams)).
 
-  Fixpoint preprocess_strpos_arg (ty : term) (s : state) {struct ty} : list bool :=
+  Fixpoint preprocess_strpos_arg (s : state) (ty : term) {struct ty} : list bool :=
     let (hd, iargs) := decompose_app ty in
     match hd with
     (* 1. If it is an product check that id does not appear left of the arrow, and check the right side *)
-    | tProd an A B => (check_not_free A s) &&l
-                      (let* _ s := add_old_var (Some "local") (mkdecl an None A) s in
-                       preprocess_strpos_arg B s)
+    | tProd an A B => (check_not_free s A) &&l
+                      (let* s _ := add_old_var s (Some "local") an A in
+                       preprocess_strpos_arg s B)
     (* 2. If it is a let in, store and check the remaining of the term *)
-    | tLetIn an A db B => let* _ s := add_old_var (Some "local") (mkdecl an None A) s in
-                          preprocess_strpos_arg (reduce_lets s B) s
+    | tLetIn an db A B => let* s _ := add_old_letin s (Some "local") an db A in
+                          preprocess_strpos_arg s (reduce_lets s B)
     (* 3. If it is variable:  *)
-    | tRel n => if check_ids n id_inds s
+    | tRel n => if check_keys s key_inds n
                 (* 3.1 If it is the inductive type being defined, then nothing to check *)
                 then default_value
                 (* 3.2 Otherwise, check the arguments  *)
-                else fold_right and_list default_value (map (fun X => check_not_free X s) iargs)
+                else fold_right and_list default_value (map (fun X => check_not_free s X) iargs)
     (* 3. If it is nested *)
     | tInd (mkInd kname_indb pos_indb) _ =>
         (* Check if there is at least one argument to save computation *)
@@ -111,12 +111,12 @@ Section CheckArg.
                 - if you can nest on it => check for strict positivity in the instantiation
                 - if you can not => check if they appear in it *)
             let strpos_uparams := fold_right (fun ' (b, X) t =>
-                if (b : bool) then preprocess_strpos_arg X s &&l t else check_not_free X s)
+                if (b : bool) then preprocess_strpos_arg s X &&l t else check_not_free s X)
               default_value (combine nestable uparams_inst) in
             (* 3.2 Check they do not appear in the instantiation of nuparams or indices *)
-              let free_nuparams_indices := fold_right (fun X t => check_not_free X s &&l t)
+              let free_nuparams_indices := fold_right (fun X t => check_not_free s X &&l t)
                                               default_value nuparams_indices_inst in
-            (* 3.3 Check they do not appear in the type of a varibale in the nuparams or indices *)
+            (* 3.3 Check they do not appear in the type of a variable in the nuparams or indices *)
             strpos_uparams &&l free_nuparams_indices
         | None => all_false
         end
@@ -125,10 +125,8 @@ Section CheckArg.
 
 
   (* Check the uparams does not appear in the types *)
-  Definition check_free_cxt : list term -> state -> list bool :=
-    fun lty s =>
-    fold_right (fun X t => check_not_free X s &&l t)
-      default_value lty.
+  Definition check_free_cxt : state -> list term -> list bool :=
+    fun s lty => fold_right (fun X t => check_not_free s X &&l t) default_value lty.
 
 End CheckArg.
 
@@ -137,34 +135,61 @@ End CheckArg.
 Definition preprocess_strpos : list bool :=
   (* add inds *)
   let s := add_mdecl kname nb_uparams mdecl init_state in
-  let* id_inds s := add_inds (get_mdecl kname s) s in
-  let* _ id_uparams _ s  := add_old_context (Some "uparams") (get_uparams kname s) s in
-  let* _ id_nuparams _ s := add_old_context (Some "nparams") (get_nuparams kname s) s in
+  let* s key_inds := add_inds (get_mdecl kname s) s in
+  let* s _ key_uparams _  := add_old_context s (Some "uparams") (get_uparams kname s)  in
+  let* s _ key_nuparams _ := add_old_context s (Some "nparams") (get_nuparams kname s) in
   (* 1. Check strict positivity in the arguments *)
-  (check_ctors_by_arg and_list default_value E (preprocess_strpos_arg id_inds id_uparams)
-    (get_all_args kname s) s)
+  (check_ctors_by_arg and_list default_value E s (preprocess_strpos_arg key_inds key_uparams)
+    (get_all_args kname s))
   (* Check the uparams does not appear in the types of the non uniform parameters *)
-  &&l (check_free_cxt id_uparams (map decl_type (get_nuparams kname s)) s)
+  &&l (check_free_cxt key_uparams s (map decl_type (get_nuparams kname s)))
   (* Check the uparams does not appear in the types of the indices *)
-  &&l (check_free_cxt id_uparams (fold_right (fun indb t => (map decl_type indb.(ind_indices)) ++ t)
-                                    [] mdecl.(ind_bodies)) s).
+  &&l (check_free_cxt key_uparams s (fold_right (fun indb t => (map decl_type indb.(ind_indices)) ++ t)
+                                    [] mdecl.(ind_bodies))).
 
 
 (* 4. Debug function *)
-Definition debug_preprocess_strpos : string * list (string * list (list bool)) :=
+Section Foo.
+
+Context (key_inds     : keys).
+Context (key_uparams  : keys).
+Context (key_nuparams : keys).
+
+#[using="All"]
+Fixpoint debug_strpos_arg (s : state) (ty : term) {struct ty} : term :=
+  let (hd, iargs) := decompose_app ty in
+  match hd with
+  (* 1. If it is an product check that id does not appear left of the arrow, and check the right side *)
+  | tProd an A B =>
+                    (let* s _ := add_old_var s (Some "local") an A in
+                     debug_strpos_arg s B)
+  (* 2. If it is a let in, store and check the remaining of the term *)
+  | tLetIn an db A B => let* s _ := add_old_letin s (Some "local") an db A in
+                        debug_strpos_arg s (reduce_lets s B)
+  (* 3. If it is variable:  *)
+  | tRel n => mkApps (tVar "DEBUG:")
+                [ state_to_term s;
+                  mkApp (tVar "var :=") (tRel n) ;
+                  mkApps (tVar "key_inds :=") (map (fun n => tRel n) key_inds);
+                  if check_keys s key_inds n then tVar "TRUE" else tVar "FALSE"
+                ]
+  (* 3. If it is nested *)
+  | tInd (mkInd kname_indb pos_indb) _ => tVar "not important"
+  | _ => tVar "not important"
+  end.
+
+End Foo.
+
+Definition debug_preprocess_strpos : string * list (string * list _) :=
   (* add inds *)
   let s := add_mdecl kname nb_uparams mdecl init_state in
-  let* id_inds s := add_inds (get_mdecl kname s) s in
-  let* _ id_uparams _ s  := add_old_context (Some "uparams") (get_uparams kname s) s in
-  let* _ id_nuparams _ s := add_old_context (Some "nparams") (get_nuparams kname s) s in
+  let* s key_inds := add_inds (get_mdecl kname s) s in
+  let* s _ key_uparams _  := add_old_context s (Some "uparams") (get_uparams kname s) in
+  let* s _ key_nuparams _ := add_old_context s (Some "nparams") (get_nuparams kname s) in
 
-  let debug_ctor := debug_check_ctors_by_arg E (preprocess_strpos_arg id_inds id_uparams)
-                      (get_all_args kname s) s in
+  let debug_ctor := debug_check_ctors_by_arg E s (preprocess_strpos_arg key_inds key_uparams)
+                      (get_all_args kname s) in
   let annot_debug_ctor := mapi (fun i c => ("Debug Constructor " ^ string_of_nat i ^ " : ", c)) debug_ctor in
-  let debug_nuparams := check_free_cxt id_uparams (map decl_type (get_nuparams kname s)) s in
-  let debug_indices  := check_free_cxt id_uparams (fold_right (fun indb t => (map decl_type indb.(ind_indices)) ++ t)
-                        [] mdecl.(ind_bodies)) s in
-  ("Debug Strictly Positve Uniform Parameters", annot_debug_ctor ++
-    [("Debug nuparams : ", [debug_nuparams])] ++ [("Debug indices : ", [debug_indices])]).
+  ("Debug Strictly Positve Uniform Parameters", annot_debug_ctor).
 
 End CustomParam.
