named_api/Recursors/recursors.v
@@ -37,27 +37,28 @@ Section GenTypes.
 
   Section MkPreds.
 
-  Context (id_uparams : list ident).
+  Context (s : state).
+  Context (key_uparams : keys).
 
   (* 1.1.1 Builds the type of the predicate for the i-th block
     forall (B0 : R0) ... (Bm : Rm),
     forall (i1 : t1) ... (il : tl),
       (Ind A1 ... An B0 ... Bm i1 ... il) -> U)  *)
-  Definition make_type_pred : nat -> state -> term :=
-    fun pos_indb s =>
-    let* id_nuparams s := closure_nuparams tProd kname s in
-    let* id_indices  s := closure_indices  tProd kname pos_indb s in
+  Definition make_type_pred : state -> nat -> term :=
+    fun s pos_indb =>
+    let* s key_nuparams := closure_nuparams tProd s kname in
+    let* s key_indices  := closure_indices  tProd s kname pos_indb in
     tProd (mkBindAnn nAnon (get_relevance kname pos_indb s))
-          (make_ind kname pos_indb id_uparams id_nuparams id_indices s)
+          (make_ind s kname pos_indb key_uparams key_nuparams key_indices)
           U.(out_univ).
 
   (* 1.2.1 Compute closure predicates *)
-  Definition closure_preds : state -> (list ident -> state -> term) -> term :=
-    fun s t =>
-    closure_binder binder (Some "preds") (get_ind_bodies kname s)
+  Definition closure_preds : (state -> keys -> term) -> term :=
+    fun cc =>
+    closure_binder binder s (Some "preds") (get_ind_bodies kname s)
       (fun pos_indb indb => mkBindAnn (nNamed (naming_pred pos_indb)) U.(out_relev))
-      (fun pos_indb indb s => make_type_pred pos_indb s)
-      s t.
+      (fun pos_indb indb s => make_type_pred s pos_indb)
+      cc.
 
   End MkPreds.
 
@@ -67,22 +68,23 @@ Section GenTypes.
 
   Section MkCtor.
 
-  Context (id_uparams : list ident).
-  Context (id_preds   : list ident).
+  Context (s : state).
+  Context (key_uparams : keys).
+  Context (key_preds   : keys).
 
   (* 1.2.1 Generates the type associated to an argument *)
   (* forall x, [P x] storing the ident correctly *)
   Definition make_type_arg : context_decl -> state ->
-      (list ident -> list ident -> list ident -> state -> term) -> term :=
-    fun '(mkdecl an db ty) s t =>
+      (state -> keys -> keys -> keys -> term) -> term :=
+    fun '(mkdecl an db ty) s cc =>
     match db with
-    | Some db => kp_tLetIn an db ty s (fun x => t [x] [] [])
-    | None => let* id_arg s := kp_tProd an ty (Some "args") s in
-              let red_ty := reduce_full E s (get_type id_arg s) in
-              match make_rec_call kname Ep id_preds [] id_arg red_ty s with
-              | Some (ty, _) => mk_tProd (mkBindAnn nAnon Relevant) ty (Some "rec_call") s
-                                  (fun id_rec => t [] [id_arg] [id_rec])
-              | None => t [] [id_arg] [] s
+    | Some db => kp_tLetIn s an db ty (fun s x => cc s [x] [] [])
+    | None => let* s key_arg := kp_tProd s (Some "args") an ty in
+              let red_ty := reduce_full E s (get_type s key_arg) in
+              match make_rec_call kname Ep s key_preds [] key_arg red_ty with
+              | Some (ty, _) => mk_tProd s (Some "rec_call") (mkBindAnn nAnon Relevant) ty
+                                  (fun s key_rec => cc s [] [key_arg] [key_rec])
+              | None => cc s [] [key_arg] []
               end
     end.
 
@@ -90,24 +92,24 @@ Section GenTypes.
   (* forall (B0 : R0) ... (Bm : Rm),
      forall x0 : t0, [P x0], ..., xn : tn, [P n],
      P B0 ... Bm f0 ... fl (cst A0 ... An B0 ... Bm x0 ... xl) *)
-  Definition make_type_ctor : nat -> constructor_body -> nat -> state -> term :=
-  fun pos_indb ctor pos_ctor s =>
-  let* id_nuparams s := closure_nuparams tProd kname s in
-  let* _ id_args _ s := fold_left_state_opt3 (fun _ => make_type_arg) ctor.(cstr_args) s in
-  mkApp (make_predn id_preds pos_indb id_nuparams (get_ctor_indices kname pos_indb pos_ctor s) s)
-        (mkApps (make_cst kname pos_indb pos_ctor id_uparams id_nuparams s)
-                (get_terms id_args s)).
+  Definition make_type_ctor : state -> nat -> constructor_body -> nat -> term :=
+  fun s pos_indb ctor pos_ctor =>
+  let* s key_nuparams := closure_nuparams tProd s kname in
+  let* s _ key_args _ := fold_left_state_opt3 (fun _ => make_type_arg) ctor.(cstr_args) s in
+  mkApp (make_predn s key_preds pos_indb key_nuparams (get_ctor_indices kname pos_indb pos_ctor s))
+        (mkApps (make_cst s kname pos_indb pos_ctor key_uparams key_nuparams)
+                (get_terms s key_args)).
 
   (* 2.3 Closure ctors of one inductive block *)
-  Definition closure_ctors_block : nat -> one_inductive_body -> state -> (list ident -> state -> term) -> term :=
-    fun pos_indb indb =>
-    closure_binder binder (Some "ctors") indb.(ind_ctors)
+  Definition closure_ctors_block : nat -> one_inductive_body -> state -> (state -> keys -> term) -> term :=
+    fun pos_indb indb s =>
+    closure_binder binder s (Some "ctors") indb.(ind_ctors)
     (fun pos_ctor ctor => mkBindAnn (nNamed (make_name_bin "f" pos_indb pos_ctor)) U.(out_relev))
-    (fun pos_ctor ctor s => make_type_ctor pos_indb ctor pos_ctor s).
+    (fun pos_ctor ctor s => make_type_ctor s pos_indb ctor pos_ctor).
 
   (* 2.4 Closure all ctors *)
-  Definition closure_ctors : state -> (list (list ident) -> state -> term) -> term :=
-    fun s t => fold_right_state closure_ctors_block (get_ind_bodies kname s) s t.
+  Definition closure_ctors : (state -> list keys -> term) -> term :=
+    fun cc => fold_right_state closure_ctors_block (get_ind_bodies kname s) s cc.
 
   End MkCtor.
 
@@ -116,29 +118,30 @@ Section GenTypes.
 
   Section MkCcl.
 
-  Context (id_uparams : list ident).
-  Context (id_preds   : list ident).
+  Context (s :state).
+  Context (key_uparams : keys).
+  Context (key_preds   : keys).
   Context (pos_indb : nat).
 
   (* 1.3.1 Make the type of the conclusion *)
   (* P B0 ... Bm i0 ... il x *)
-  Definition make_ccl : list ident -> list ident -> ident -> state -> term :=
-    fun id_nuparams id_indices id_VarMatch s =>
-    mkApp (make_predn id_preds pos_indb id_nuparams (get_terms id_indices s) s)
-          (get_term id_VarMatch s).
+  Definition make_ccl : state -> keys -> keys -> key -> term :=
+    fun s key_nuparams key_indices key_VarMatch =>
+    mkApp (make_predn s key_preds pos_indb key_nuparams (get_terms s key_indices))
+          (get_term s key_VarMatch).
 
   (* 1.3.2 Make the return type *)
   (* forall (B0 : R0) ... (Bm : Rm),
      forall (i1 : t1) ... (il : tl),
      forall (x : Ind A0 ... An B0 ... Bm i0 ... il),
       P B0 ... Bm i0 ... il x *)
-  Definition make_return_type : state -> term :=
-    fun s =>
-    let* id_nuparams s := closure_nuparams tProd kname s in
-    let* id_indices  s := closure_indices  tProd kname pos_indb s in
-    let* id_VarMatch s := mk_tProd (mkBindAnn (nNamed "x") (get_relevance kname pos_indb s))
-                            (make_ind kname pos_indb id_uparams id_nuparams id_indices s) (Some "VarMatch") s in
-    make_ccl id_nuparams id_indices id_VarMatch s.
+  Definition make_return_type : term :=
+    let* s key_nuparams := closure_nuparams tProd s kname in
+    let* s key_indices  := closure_indices  tProd s kname pos_indb in
+    let* s key_VarMatch := mk_tProd s (Some "VarMatch")
+                            (mkBindAnn (nNamed "x") (get_relevance kname pos_indb s))
+                            (make_ind s kname pos_indb key_uparams key_nuparams key_indices) in
+    make_ccl s key_nuparams key_indices key_VarMatch.
 
   End MkCcl.
 
@@ -152,11 +155,11 @@ Section GenTypes.
 
 Definition gen_rec_type (pos_indb : nat) : term :=
   let s := add_mdecl kname nb_uparams mdecl init_state in
-  let* s := replace_ind kname s in
-  let* id_uparams s := closure_uparams tProd kname s in
-  let* id_preds   s := closure_preds   tProd id_uparams s in
-  let* id_ctors   s := closure_ctors   tProd id_uparams id_preds s in
-  make_return_type id_uparams id_preds pos_indb s.
+  let* s := replace_ind s kname in
+  let* s key_uparams := closure_uparams tProd s kname in
+  let* s key_preds   := closure_preds   tProd s key_uparams in
+  let* s key_ctors   := closure_ctors   tProd s key_uparams key_preds in
+  make_return_type s key_uparams key_preds pos_indb.
 
 
 
@@ -167,18 +170,19 @@ Definition gen_rec_type (pos_indb : nat) : term :=
 (* 3.1 Compute the arguments of the rec call *)
 Section GetRecCall.
 
-  Context (id_preds : list ident).
-  Context (id_fixs : list ident).
+  Context (s : state).
+  Context (key_preds : keys).
+  Context (key_fixs  : keys).
 
-  Definition compute_args_fix : list ident -> state -> list term :=
-    fun id_args s =>
-    fold_right (fun id_arg t =>
-      let red_ty := reduce_full E s (get_type id_arg s) in
-      match make_rec_call kname Ep id_preds id_fixs id_arg red_ty s with
-      | Some (rc_ty, rc_tm) => (get_term id_arg s) :: rc_tm :: t
-      | None => (get_term id_arg s) :: t
+  Definition compute_args_fix : keys -> list term :=
+    fun key_args =>
+    fold_right (fun key_arg t =>
+      let red_ty := reduce_full E s (get_type s key_arg) in
+      match make_rec_call kname Ep s key_preds key_fixs key_arg red_ty with
+      | Some (rc_ty, rc_tm) => (get_term s key_arg) :: rc_tm :: t
+      | None => (get_term s key_arg) :: t
       end
-    ) [] id_args.
+    ) [] key_args.
 
 End GetRecCall.
 
@@ -187,28 +191,30 @@ End GetRecCall.
 Definition gen_rec_term (pos_indb : nat) : term :=
   (* 0. Initialise state with inductives *)
   let s := add_mdecl kname nb_uparams mdecl init_state in
-  let* s := replace_ind kname s in
+  let* s := replace_ind s kname in
   (* 1. Closure Uparams / preds / ctors *)
-  let* id_uparams s := closure_uparams tLambda kname s in
-  let* id_preds   s := closure_preds tLambda id_uparams s in
-  let* id_ctors   s := closure_ctors tLambda id_uparams id_preds s in
+  let* s key_uparams := closure_uparams tLambda s kname in
+  let* s key_preds   := closure_preds   tLambda s key_uparams in
+  let* s key_ctors   := closure_ctors   tLambda s key_uparams key_preds in
   (* 2. Fixpoint *)
-  let tFix_type pos_indb := make_return_type id_uparams id_preds pos_indb s in
-  let tFix_rarg := tFix_default_rarg kname s in
-  let* id_fixs pos_indb s := mk_tFix kname tFix_type tFix_rarg pos_indb s in
+  let tFix_type pos_indb := make_return_type s key_uparams key_preds pos_indb in
+  let tFix_rarg := tFix_default_rarg s kname in
+  let* s key_fixs pos_indb := mk_tFix kname tFix_type tFix_rarg s pos_indb in
   (* 3. Closure Nuparams / Indices / Var *)
-  let* id_nuparams s := closure_nuparams tLambda kname s in
-  let* id_indices  s := closure_indices tLambda kname pos_indb s in
-  let* id_VarMatch s := mk_tLambda (mkBindAnn (nNamed "x") Relevant)
-                        (make_ind kname pos_indb id_uparams id_nuparams id_indices s)
-                        (Some "VarMatch") s in
+  let* s key_nuparams := closure_nuparams tLambda s kname in
+  let* s key_indices  := closure_indices  tLambda s kname pos_indb in
+  let* s key_VarMatch := mk_tLambda s (Some "VarMatch")
+                        (mkBindAnn (nNamed "x") Relevant)
+                        (make_ind s kname pos_indb key_uparams key_nuparams key_indices) in
   (* 4. Proof of P ... x by match *)
-  let tCase_pred := make_ccl id_preds pos_indb id_nuparams in
-  let* pos_ctor ctor id_args _ s := mk_tCase kname pos_indb
-          tCase_pred id_uparams id_nuparams (get_term id_VarMatch s) s in
+  let tCase_pred := (fun s => make_ccl key_preds pos_indb s key_nuparams) in
+  let* s _ key_args _ pos_ctor := mk_tCase kname pos_indb
+          tCase_pred key_uparams key_nuparams s (get_term s key_VarMatch) in
   (* 5. Make the branch *)
-  (mkApps (getij_term id_ctors pos_indb pos_ctor s)
-          (get_terms id_nuparams s ++ compute_args_fix id_preds id_fixs id_args s)).
+  (mkApps (getij_term s key_ctors pos_indb pos_ctor)
+          (get_terms s key_nuparams ++ compute_args_fix s key_preds key_fixs key_args)).
+            (* [state_to_term s])). *)
+
 
 
 End GenRecursors.
