named_api/UnitTests/t06_lets_and_reduction.v
@@ -16,8 +16,8 @@ Inductive b_let_param1 A (PA : A -> Prop) : b_let A -> Type :=
 
 
 MetaCoq Run (tmMsg "01/10 btlet").
-Redirect "UnitTests/tests/06_01_b_let_coq" MetaCoq Run (print_rec "b_let").
-Redirect "UnitTests/tests/06_01_b_let_gen" MetaCoq Run (generate Ep b_let).
+Redirect "named_api/UnitTests/tests/06_01_b_let_coq" MetaCoq Run (print_rec "b_let").
+Redirect "named_api/UnitTests/tests/06_01_b_let_gen" MetaCoq Run (generate Ep b_let).
 
 Inductive rc_let (A : Type) : Type :=
 | rc_letz : rc_let A
@@ -31,8 +31,8 @@ Inductive rc_let_param1 A (PA : A -> Prop) : rc_let A -> Type :=
                    rc_let_param1 A PA (rc_lets A a x).
 
 MetaCoq Run (tmMsg "02/10 rc_let").
-Redirect "UnitTests/tests/06_02_rc_let_coq" MetaCoq Run (print_rec "rc_let").
-Redirect "UnitTests/tests/06_02_rc_let_gen" MetaCoq Run (generate Ep rc_let).
+Redirect "named_api/UnitTests/tests/06_02_rc_let_coq" MetaCoq Run (print_rec "rc_let").
+Redirect "named_api/UnitTests/tests/06_02_rc_let_gen" MetaCoq Run (generate Ep rc_let).
 
 Inductive rc_letpar (A : Prop) : Type :=
 | rc_letparz : rc_letpar A
@@ -46,8 +46,8 @@ Inductive rc_letpar_param1 A (PA : A -> Prop) : rc_letpar A -> Type :=
                       rc_letpar_param1 A PA (rc_letpars A n m x z).
 
 MetaCoq Run (tmMsg "03/10 re_letpar").
-Redirect "UnitTests/tests/06_03_rc_letpar_coq" MetaCoq Run (print_rec "rc_letpar").
-Redirect "UnitTests/tests/06_03_rc_letpar_gen" MetaCoq Run (generate Ep rc_letpar).
+Redirect "named_api/UnitTests/tests/06_03_rc_letpar_coq" MetaCoq Run (print_rec "rc_letpar").
+Redirect "named_api/UnitTests/tests/06_03_rc_letpar_gen" MetaCoq Run (generate Ep rc_letpar).
 
 Inductive crazy1 : nat -> Type :=
 | crazy1_z : crazy1 0
@@ -58,8 +58,8 @@ Inductive crazy1_param1 : forall n, crazy1 n -> Type :=
 | crazy1_s_param1 : forall n x, crazy1_param1 n x.
 
 MetaCoq Run (tmMsg "04/10 crazy1").
-Redirect "UnitTests/tests/06_04_crazy1_coq" MetaCoq Run (print_rec "crazy1").
-Redirect "UnitTests/tests/06_04_crazy1_gen" MetaCoq Run (generate Ep crazy1).
+Redirect "named_api/UnitTests/tests/06_04_crazy1_coq" MetaCoq Run (print_rec "crazy1").
+Redirect "named_api/UnitTests/tests/06_04_crazy1_gen" MetaCoq Run (generate Ep crazy1).
 
 Inductive crazy2 (A : let y := Prop in y + Prop) : (let y := bool in bool + nat) -> Type :=
 | crazy2_z : crazy2 A (inr 0)
@@ -74,8 +74,8 @@ Inductive crazy2_param1 (A : let y := Prop in y + Prop) : forall z, crazy2 A z -
                     crazy2_param1 A (let y := 0 in inr (x + y)) (crazy2_s A k n m Hm Hm1 c).
 
 MetaCoq Run (tmMsg "05/10 crazy2").
-Redirect "UnitTests/tests/06_05_crazy2_coq" MetaCoq Run (print_rec "crazy2").
-Redirect "UnitTests/tests/06_05_crazy2_gen" MetaCoq Run (generate Ep crazy2).
+Redirect "named_api/UnitTests/tests/06_05_crazy2_coq" MetaCoq Run (print_rec "crazy2").
+Redirect "named_api/UnitTests/tests/06_05_crazy2_gen" MetaCoq Run (generate Ep crazy2).
 
 Inductive diag : term -> term -> Type :=
 | dcons c : diag c c -> let ptm := c in diag c c.
@@ -87,8 +87,8 @@ Inductive diag_param1 : forall t1 t2, diag t1 t2 -> Type :=
                  diag_param1 c c (dcons c x).
 
 MetaCoq Run (tmMsg "06/10 diag").
-Redirect "UnitTests/tests/06_06_diag_coq" MetaCoq Run (print_rec "diag").
-Redirect "UnitTests/tests/06_06_diag_gen" MetaCoq Run (generate Ep diag).
+Redirect "named_api/UnitTests/tests/06_06_diag_coq" MetaCoq Run (print_rec "diag").
+Redirect "named_api/UnitTests/tests/06_06_diag_gen" MetaCoq Run (generate Ep diag).
 
 Inductive redc : nat -> Type :=
 | redc0 : redc 0
@@ -101,8 +101,8 @@ Inductive redc_param1 : forall n, redc n -> Type :=
                  redc_param1 n (redc1 n x).
 
 MetaCoq Run (tmMsg "07/10 redc").
-Redirect "UnitTests/tests/06_07_redc_coq" MetaCoq Run (print_rec "redc").
-Redirect "UnitTests/tests/06_07_redc_gen" MetaCoq Run (generate Ep redc).
+Redirect "named_api/UnitTests/tests/06_07_redc_coq" MetaCoq Run (print_rec "redc").
+Redirect "named_api/UnitTests/tests/06_07_redc_gen" MetaCoq Run (generate Ep redc).
 
 Definition foo : Type -> Type := fun x => x.
 
@@ -117,8 +117,8 @@ Inductive redEnv_param1 : redEnv -> Type :=
                    redEnv_param1 (redEnv1 x y).
 
 MetaCoq Run (tmMsg "08/10 redEnv").
-Redirect "UnitTests/tests/06_08_redEnv_coq" MetaCoq Run (print_rec "redEnv").
-Redirect "UnitTests/tests/06_08_redEnv_gen" MetaCoq Run (generate Ep redEnv).
+Redirect "named_api/UnitTests/tests/06_08_redEnv_coq" MetaCoq Run (print_rec "redEnv").
+Redirect "named_api/UnitTests/tests/06_08_redEnv_gen" MetaCoq Run (generate Ep redEnv).
 
 Inductive nu_let1 (A : Type) : Type :=
 | nu_let1_nil : nu_let1 A
@@ -130,8 +130,8 @@ Inductive nu_let1_param1 A (PA : A -> Type) : nu_let1 A -> Type :=
                         nu_let1_param1 A PA (nu_let1_cons A z).
 
 MetaCoq Run (tmMsg "09/10 nu_let1").
-Redirect "UnitTests/tests/06_09_nu_let1_coq" MetaCoq Run (print_rec "nu_let1").
-Redirect "UnitTests/tests/06_09_nu_let1_gen" MetaCoq Run (generate Ep nu_let1).
+Redirect "named_api/UnitTests/tests/06_09_nu_let1_coq" MetaCoq Run (print_rec "nu_let1").
+Redirect "named_api/UnitTests/tests/06_09_nu_let1_gen" MetaCoq Run (generate Ep nu_let1).
 
 Inductive nu_let2 (A : Type) : Type :=
 | nu_let2_nil : nu_let2 A
@@ -143,5 +143,5 @@ Inductive nu_let2_param1 A : nu_let2 A -> Type :=
                         nu_let2_param1 A (nu_let2_cons A z).
 
 MetaCoq Run (tmMsg "10/10 nu_let2").
-Redirect "UnitTests/tests/06_10_nu_let2_coq" MetaCoq Run (print_rec "nu_let2").
-Redirect "UnitTests/tests/06_10_nu_let2_gen" MetaCoq Run (generate Ep nu_let2).
+Redirect "named_api/UnitTests/tests/06_10_nu_let2_coq" MetaCoq Run (print_rec "nu_let2").
+Redirect "named_api/UnitTests/tests/06_10_nu_let2_gen" MetaCoq Run (generate Ep nu_let2).
